

Solution - Midterm Test Algebra 2

Exercise 1:

1/ $A = 2I_3 + J$ where $J = \begin{pmatrix} 0 & 1 & 0 \\ 0 & 0 & 1 \\ 0 & 0 & 0 \end{pmatrix}$

$J^2 = \begin{pmatrix} 0 & 0 & 1 \\ 0 & 0 & 0 \\ 0 & 0 & 0 \end{pmatrix}$, $J^3 = O_3$, $J^k = O$ for $k \geq 3$.

$$A^k = (2I_3 + J)^k = \sum_{i=0}^k \binom{k}{i} 2^{k-i} J^i$$

$$= \sum_{i=0}^k \binom{k}{i} 2^{k-i} J^i$$

$$A^k = \begin{pmatrix} 2^k & k 2^{k-1} & k(k-1) 2^{k-3} \\ 0 & 2^k & k 2^{k-1} \\ 0 & 0 & 2^k \end{pmatrix}$$

2) $P(X) = \sum_{k=0}^{\infty} \frac{P^{(k)}(2)}{k!} (X-2)^k$

$$P(A) = \sum_{k=0}^{\infty} \frac{P^{(k)}(2)}{k!} (A-2I)^k$$

$$= \sum_{k=0}^{\infty} \frac{P^{(k)}(2)}{k!} J^k$$

$$= P(2) I_2 + P'(2) J + \frac{1}{2} P''(2) J^2 \quad (J^k = O \text{ for } k \geq 3)$$

$$= \begin{pmatrix} P(2) & P'(2) & \frac{1}{2} P''(2) \\ 0 & P(2) & P'(2) \\ 0 & 0 & P(2) \end{pmatrix}$$

Exercise 2:

1/ $P(A) = A^2 - A = A - A = 0 \Rightarrow P$ is an annihilating polynomial for A . (0,5)

* Suppose that A is invertible. We have,

$$A \cdot A^{-1} = I \Rightarrow A^2 A^{-1} = A$$

(0,5)

$$\begin{aligned} A^2 A^{-1} - A A^{-1} &= A - I \Rightarrow (A^2 - A) A^{-1} = A - I \\ &\Rightarrow P(A) A^{-1} = A - I \\ &\Rightarrow A = I \text{ contradiction} \end{aligned}$$

* Suppose that $A - I$ is invertible.

$$\begin{aligned} P(A) = A^2 - A = 0 &\Rightarrow A(A - I) = 0 \\ &\Rightarrow A(A - I)(A - I)^{-1} = 0 \cdot (A - I)^{-1} = 0 \\ &\Rightarrow A = 0 \text{ Contradiction.} \end{aligned}$$

(0,5)

2) $A = \begin{pmatrix} 3 & -1 \\ 6 & -2 \end{pmatrix} \sim \begin{pmatrix} 3 & -1 \\ 0 & 0 \end{pmatrix} R_2 \leftarrow R_2 - 2R_1$

A is in row echelon form with one zero entry in his diagonal. So A is not invertible. (0,5)

3) We have $C_3 = -3C_2 \Rightarrow A$ is not invertible.

Or: $R_2 = 2R_1$

$\Rightarrow A$ is not invertible

Or: $\det A = 0 \Rightarrow A$ is not invertible

(0,5)

Exercise 3:

1/ $K^2 = -I_4$ (0,25)

$$K(-K) = I_4 \Rightarrow K \text{ is invertible with } K^{-1} = -K.$$

(0,25)

(0,25)

(0,25)

2/ We have $aI \cdot bK = bK \cdot aI$

$$\text{Then: } L^2 = (aI + bK)^2 = a^2I + b^2K^2 + 2abK$$

$$= a^2I - b^2I + 2abK$$

$$= a^2I - b^2I + 2a(bK + aI) - 2a^2I$$

$$= -a^2I - b^2I + 2aL$$

$$= -(a^2 + b^2)I + 2aL$$

(1)

3/ We have a and b are not both zero $\Rightarrow a^2 + b^2 \neq 0$.

$$L^2 = -(a^2 + b^2)I + 2aL \Rightarrow L^2 - 2aL = -(a^2 + b^2)I$$

$$\Rightarrow L \left(-\frac{1}{a^2 + b^2} (L - 2aI) \right) = I$$

$\Rightarrow L$ is invertible with:

$$L^{-1} = -\frac{1}{a^2 + b^2} L + \frac{2a}{a^2 + b^2} I$$

$$\Rightarrow L^{-1} = \underbrace{\frac{a}{a^2 + b^2}}_c I - \underbrace{\frac{b}{a^2 + b^2}}_d K$$

$$= cI + dK$$

$$4) A = \sqrt{2}I + K \Rightarrow A^{-1} = \frac{\sqrt{2}}{(\sqrt{2})^2 + (1)^2} I - \frac{1}{3} K$$

$$= \frac{\sqrt{2}}{3} I - \frac{1}{3} K$$

$$A^{-1} = \begin{pmatrix} \frac{\sqrt{2}-1}{3} & -\frac{1}{3} & \frac{1}{3} & 1 \\ -\frac{1}{3} & \frac{\sqrt{2}-1}{3} & -\frac{1}{3} & \frac{2}{3} \\ 0 & \frac{1}{3} & \frac{\sqrt{2}}{3} & -\frac{1}{3} \\ -\frac{1}{3} & -\frac{1}{3} & 0 & \frac{\sqrt{2}+2}{3} \end{pmatrix}$$

Exercise 4:

1. a) Let $\alpha, \beta \in \mathbb{R}$

$$\alpha \cdot 1 + \beta \cdot i = 0 \Rightarrow \alpha = \beta = 0.$$

(0,75)

The \mathbb{F} is linearly independent.

b) We have: $\alpha \cdot 1 + \beta \cdot i = 0$ for $\alpha = i$ and $\beta = -1 \neq 0$.

So \mathbb{F} is linearly dependent.

(0,75)

2. a) * $\mathbb{R} \cdot w \subset \mathcal{C}$ (0,25)

$$* 0_{\mathcal{C}} = 0_{\mathbb{R}} \cdot w \in \mathbb{R} \cdot w$$

(0,25)

* Let $u, v \in \mathbb{R} \cdot w$ and $\alpha, \beta \in \mathbb{R}$

$$u \in \mathbb{R} \cdot w \Rightarrow u = x \cdot w, \quad x \in \mathbb{R}$$

$$v \in \mathbb{R} \cdot w \Rightarrow v = x' \cdot w, \quad x' \in \mathbb{R}$$

$$\alpha u + \beta v = \alpha x \cdot w + \beta x' \cdot w$$

$$= \underbrace{(\alpha x + \beta x')}_{\in \mathbb{R}} \cdot w \in \mathbb{R} \cdot w$$

(1)

Then $\mathbb{R} \cdot w$ is a subspace of the \mathbb{R} -vector space \mathcal{C} .

b) When \mathcal{C} is considered as a \mathbb{C} -vector space,

$\mathbb{R} \cdot w$ is a subspace of \mathcal{C} if and only if $w = 0$.

In this case, $\mathbb{R} \cdot w = \{0\}$ is the only subspace of \mathcal{C} .

(1)

Exercise 5:

1) * $F \subset \mathcal{C}^2(\mathbb{R}, \mathbb{R})$ (0,25)

$$* 0_{\mathcal{C}^2(\mathbb{R}, \mathbb{R})} \in F \quad \text{because: } \left(0_{\mathcal{C}^2(\mathbb{R}, \mathbb{R})}\right)' = 0 = (1+x^2) \cdot 0_{\mathcal{C}^2(\mathbb{R}, \mathbb{R})}$$

(0,25)

* Let $\varphi_1, \varphi_2 \in F$ and $\alpha, \beta \in \mathbb{R}$

$$\text{We denote: } \psi = \alpha \varphi_1 + \beta \varphi_2$$

$$\begin{aligned}
 \psi''(x) &= \alpha \psi_1''(x) + \beta \psi_2''(x) \\
 &= \alpha (1+x^2) \psi_1(x) + \beta (1+x^2) \psi_2(x) \\
 &= (1+x^2) (\alpha \psi_1(x) + \beta \psi_2(x)) \\
 &= (1+x^2) \psi(x)
 \end{aligned}$$

1

Then F is a subspace of $\mathcal{C}^2(\mathbb{R}, \mathbb{R})$.

$$\begin{aligned}
 2) \quad v, w \in F &\Rightarrow v''(x) = (1+x^2) v(x) \\
 &\quad w''(x) = (1+x^2) w(x)
 \end{aligned}$$

$$\begin{aligned}
 (v w' - w v')' &= \cancel{v' w'} + v w'' - \cancel{w' v'} - w v'' \\
 &= v(1+x^2)w - w(1+x^2)v \\
 &= (1+x^2)(vw - wv) \\
 &= 0
 \end{aligned}$$

01

Then $v w' - w v'$ is constant on \mathbb{R} .

3) Show that $f, g \in F$.

We have, $f'(x) = x e^{\frac{x^2}{2}}$

$$f''(x) = e^{\frac{x^2}{2}} + x^2 e^{\frac{x^2}{2}} = (1+x^2) e^{\frac{x^2}{2}} = (1+x^2) f(x)$$

01

So $f \in F$

$$\begin{aligned}
 g'(x) &= x e^{\frac{x^2}{2}} \int_0^x e^{-t^2} dt + e^{\frac{x^2}{2}} \left(\int_0^x e^{-t^2} dt \right)' \\
 &= x e^{\frac{x^2}{2}} \int_0^x e^{-t^2} dt + e^{\frac{x^2}{2}} e^{-x^2} \\
 &= x e^{\frac{x^2}{2}} \int_0^x e^{-t^2} dt + e^{-\frac{x^2}{2}}
 \end{aligned}$$

$$\begin{aligned}
 g''(x) &= x \left[x e^{\frac{x^2}{2}} \int_0^x e^{-t^2} dt + e^{-\frac{x^2}{2}} \right] + e^{\frac{x^2}{2}} \int_0^x e^{-t^2} dt - x e^{\frac{x^2}{2}} \\
 &= x^2 e^{\frac{x^2}{2}} \int_0^x e^{-t^2} dt + \cancel{x e^{\frac{x^2}{2}}} + e^{\frac{x^2}{2}} \int_0^x e^{-t^2} dt - \cancel{x e^{\frac{x^2}{2}}} \\
 &= (x^2 + 1) \left[e^{\frac{x^2}{2}} \int_0^x e^{-t^2} dt \right] \\
 &= (x^2 + 1) g(x)
 \end{aligned}$$

0,5

Then $g \in F$.

* $\{f, g\}$ is linearly independent $\Leftrightarrow \forall \alpha, \beta \in \mathbb{R}$:

$$\alpha f + \beta g = 0 \Rightarrow \alpha = \beta = 0$$

We evaluate $\alpha f + \beta g$ at 0:

$$\begin{aligned}
 \alpha f(0) + \beta g(0) &= 0 \Rightarrow \alpha + \beta \cdot 0 = 0 \\
 &\Rightarrow \alpha = 0
 \end{aligned}$$

0,5

$$\text{Then: } \beta e^{\frac{x^2}{2}} \int_0^x e^{-t^2} dt = 0 \Rightarrow \beta = 0.$$

Because $e^{\frac{x^2}{2}} > 0$ and $\int_0^x e^{-t^2}$ is strictly positive or negative.

So $\{f, g\}$ is linearly independent.

4) We have $f(x) = e^{\frac{x^2}{2}} \neq 0$.

$$\left(\frac{h}{f} \right)' = \frac{f h' - h f'}{f^2} = \frac{b}{f^2}$$

$$\frac{h}{f} = a + b \frac{g}{f} \Rightarrow \left(\frac{h}{f} \right)' = b \left(\frac{g}{f} \right)'$$

1,5

We have: $\left(\frac{g}{f} \right)' = \frac{1}{f^2}$, then there exist a and $b \in \mathbb{R}$ such that:

$$\frac{h}{f} = a + b \frac{g}{f}.$$

Then: $h = af + bg$.

5) From 4, we have: $h \in F \Rightarrow h \in \text{Span}\{f, g\}$.

So: $F \subset \text{Span}\{f, g\}$ (0,1)

It is obvious that $\text{Span}\{f, g\} \subset F$

Then: $F = \text{Span}\{f, g\}$ (0,2)

Moreover, from 3) $\{f, g\}$ is linearly independent.

It follows that $\{f, g\}$ is a basis for F . (0,2)

Finally $\dim F = 2$. (0,1)